unsafe

Phi_Semantics/PhiSem_CF_Routine.thy
@@ -2,7 +2,34 @@ theory PhiSem_CF_Routine
   imports PhiSem_CF_Break PhiSem_CF_Routine_Basic
 begin
 
+text \<open>Based on the basic routine module, we provide the version that supports return statement.\<close>
+
 declare [[\<phi>hide_techinicals = false]]
+
+definition RETURN_FRAME :: \<open>'rets::FIX_ARITY_VALs itself \<Rightarrow> RES.brk_label \<Rightarrow> bool\<close>
+  where \<open>RETURN_FRAME _ label \<longleftrightarrow> True\<close>
+
+lemma RETURN_FRAME_normal:
+  \<open> RETURN_FRAME TYPE('rets) label
+\<Longrightarrow> \<p>\<r>\<o>\<c> (op_break TYPE('any) TYPE('rets) label ret) \<lbrace> Y ret\<heavy_comma> TECHNICAL Brk_Frame label \<longmapsto> 0 \<rbrace>
+    \<t>\<h>\<r>\<o>\<w>\<s> (\<lambda>_. Brking_Frame label Y) \<close>
+  for ret :: \<open>'rets::FIX_ARITY_VALs \<phi>arg\<close>
+  using op_break_\<phi>app .
+
+lemma RETURN_FRAME_unit:
+  \<open> RETURN_FRAME TYPE(unit) label
+\<Longrightarrow> \<p>\<r>\<o>\<c> (op_break TYPE('any) TYPE(unit) label (\<phi>arg ())) \<lbrace> Y\<heavy_comma> TECHNICAL Brk_Frame label \<longmapsto> 0 \<rbrace>
+    \<t>\<h>\<r>\<o>\<w>\<s> (\<lambda>_. Brking_Frame label (\<lambda>_::unit \<phi>arg. Y)) \<close>
+  using op_break_\<phi>app[where S=\<open>\<lambda>_::unit \<phi>arg. Y\<close>] .
+
+attribute_setup RETURN_FRAME = \<open>Scan.succeed (Thm.rule_attribute [] (fn _ => fn th =>
+                    @{thm' RETURN_FRAME_unit} RS th
+    handle THM _ => @{thm' RETURN_FRAME_normal} RS th ) )\<close>
+
+
+
+
+
 
 proc op_routine:
   requires Ty_X: \<open>\<phi>_Have_Types X TY_ARGs\<close>
@@ -30,6 +57,13 @@ proc op_routine:
   \<medium_right_bracket>
 \<medium_right_bracket> .
 
+thm op_break_\<phi>app
+
+lemma
+  \<open>\<forall>ret :: unit \<phi>arg. \<p>\<r>\<o>\<c> (op_break TYPE('rets) TYPE('rets) label_ret ret) \<lbrace> Y ret\<heavy_comma> TECHNICAL Brk_Frame label_ret \<longmapsto> 0 \<rbrace>
+                      \<t>\<h>\<r>\<o>\<w>\<s> (\<lambda>_. Brking_Frame label_ret Y)
+ \<equiv> \<close>
+
 thm op_routine_\<phi>app
 
 abbreviation
@@ -43,5 +77,6 @@ attribute_setup routine =
           (fn N => fn wrap => fn Tm => Abs("label_ret", \<^typ>\<open>RES.brk_label\<close>, wrap (Tm $ Bound N)))
           @{thm "op_routine_\<phi>app"}))\<close>
 
+hide_fact RETURN_FRAME_normal
 
 end
