Phi_Semantics/PhiSem_Mem_C_Ar_MI.thy
@@ -5,53 +5,40 @@ begin
 section \<open>Pointer Arithmetic\<close>
 
 proc op_add_ptr[\<phi>overload +]:
-  input  \<open>i \<Ztypecolon> \<v>\<a>\<l> \<Ss>\<Pp>\<t>\<r>[addr:base:len] TY\<heavy_comma> j \<Ztypecolon> \<v>\<a>\<l> \<int>('b)\<close>
+  input  \<open>i \<Ztypecolon> \<v>\<a>\<l> \<Ss>\<Pp>\<t>\<r>[addr:len] TY\<heavy_comma> j \<Ztypecolon> \<v>\<a>\<l> \<int>('b)\<close>
   premises \<open>0 \<le> int i + j \<and> nat (int i + j) \<le> len\<close>
-  output \<open>nat (int i + j) \<Ztypecolon> \<v>\<a>\<l> \<Ss>\<Pp>\<t>\<r>[addr:base:len] TY\<close>
+  output \<open>nat (int i + j) \<Ztypecolon> \<v>\<a>\<l> \<Ss>\<Pp>\<t>\<r>[addr:len] TY\<close>
 \<medium_left_bracket>
   $i semantic_local_value \<open>pointer\<close>
   $j semantic_local_value \<open>\<i>\<n>\<t>('b)\<close> 
 
-  thm useful
-  from \<open>valid_logaddr_range TY addr base len\<close>[unfolded valid_logaddr_range_def]
-  have t1[useful]: \<open>valid_logaddr addr \<and> (\<forall>i<len. valid_logaddr (addr \<tribullet>\<^sub>a (base + i)\<^sup>\<t>\<^sup>\<h>) \<and> logaddr_type (addr \<tribullet>\<^sub>a (base + i)\<^sup>\<t>\<^sup>\<h>) = TY)\<close> by simp
-
-  from \<open>valid_logaddr_range TY addr base len\<close>[unfolded valid_logaddr_range_def]
-  obtain N where t2[useful]: \<open>logaddr_type addr = \<a>\<r>\<r>\<a>\<y>[N] TY\<close> and t3[useful]: \<open>base + len \<le> N\<close> by blast
-
   have [simp]: \<open>word_of_nat (nat (2 ^ LENGTH('b) + j)) = (word_of_int j :: 'b word)\<close>
-    by (smt (verit, del_insts) More_Word.power_not_zero diff_less exp_eq_zero_iff len_gt_0 less_Suc0 nat_0_le of_int_of_nat_eq power_increasing_iff the_\<phi>lemmata(4) wi_hom_add word_arith_wis(7) word_of_int_2p_len) ;;
+    by (smt (verit, ccfv_SIG) More_Word.power_not_zero diff_less int_nat_eq len_gt_0 of_int_of_nat_eq power_increasing_iff power_overflow the_\<phi>lemmata(5) word_of_int_0 word_of_int_2p_len word_of_int_hom_syms(1) zero_less_Suc) ;;
 
   semantic_return \<open>
       V_pointer.mk (V_pointer.dest (\<phi>arg.dest \<a>\<r>\<g>1)
               ||+ Word.scast (of_nat (snd (V_int.dest (\<phi>arg.dest \<a>\<r>\<g>2))) :: 'b word) * of_nat (MemObj_Size TY))
-          \<Turnstile> (nat (int i + j) \<Ztypecolon> \<Ss>\<Pp>\<t>\<r>[addr:base:len] TY)\<close>
-  certified by (insert useful, auto simp: logaddr_to_raw_array_GEP[OF t2] distrib_right,
+          \<Turnstile> (nat (int i + j) \<Ztypecolon> \<Ss>\<Pp>\<t>\<r>[addr:len] TY)\<close>
+  certified by (insert useful, auto simp: logaddr_to_raw_array_GEP[OF \<open>logaddr_type addr = \<a>\<r>\<r>\<a>\<y>[len] TY\<close>] distrib_right,
                 metis signed_of_int signed_take_bit_int_eq_self_iff the_\<phi>lemmata(4))
 \<medium_right_bracket> .
 
 
 proc (nodef) op_add_ptr_N[\<phi>overload +]:
-  input  \<open>i \<Ztypecolon> \<v>\<a>\<l> \<Ss>\<Pp>\<t>\<r>[addr:base:len] TY\<heavy_comma> j \<Ztypecolon> \<v>\<a>\<l> \<nat>('b)\<close>
+  input  \<open>i \<Ztypecolon> \<v>\<a>\<l> \<Ss>\<Pp>\<t>\<r>[addr:len] TY\<heavy_comma> j \<Ztypecolon> \<v>\<a>\<l> \<nat>('b)\<close>
   premises \<open>i + j \<le> len\<close>
-  output \<open>i + j \<Ztypecolon> \<v>\<a>\<l> \<Ss>\<Pp>\<t>\<r>[addr:base:len] TY\<close>
+  output \<open>i + j \<Ztypecolon> \<v>\<a>\<l> \<Ss>\<Pp>\<t>\<r>[addr:len] TY\<close>
 \<medium_left_bracket>
   $i semantic_local_value \<open>pointer\<close>
-  $j semantic_local_value \<open>\<i>\<n>\<t>('b)\<close> 
-
-  thm useful
-  from \<open>valid_logaddr_range TY addr base len\<close>[unfolded valid_logaddr_range_def]
-  have t1[useful]: \<open>valid_logaddr addr \<and> (\<forall>i<len. valid_logaddr (addr \<tribullet>\<^sub>a (base + i)\<^sup>\<t>\<^sup>\<h>) \<and> logaddr_type (addr \<tribullet>\<^sub>a (base + i)\<^sup>\<t>\<^sup>\<h>) = TY)\<close> by simp
-
-  from \<open>valid_logaddr_range TY addr base len\<close>[unfolded valid_logaddr_range_def]
-  obtain N where t2[useful]: \<open>logaddr_type addr = \<a>\<r>\<r>\<a>\<y>[N] TY\<close> and t3[useful]: \<open>base + len \<le> N\<close> by blast ;;
+  $j semantic_local_value \<open>\<i>\<n>\<t>('b)\<close>
 
   semantic_return \<open>
       V_pointer.mk (V_pointer.dest (\<phi>arg.dest \<a>\<r>\<g>1)
               ||+ Word.ucast (of_nat (snd (V_int.dest (\<phi>arg.dest \<a>\<r>\<g>2))) :: 'b word) * of_nat (MemObj_Size TY))
-          \<Turnstile> (i + j \<Ztypecolon> \<Ss>\<Pp>\<t>\<r>[addr:base:len] TY)\<close>
-  certified by (insert useful, auto simp: logaddr_to_raw_array_GEP[OF t2] distrib_right ucast_of_nat_small)
-
+          \<Turnstile> (i + j \<Ztypecolon> \<Ss>\<Pp>\<t>\<r>[addr:len] TY)\<close>
+  certified by (insert useful,
+                auto simp: logaddr_to_raw_array_GEP[OF \<open>logaddr_type addr = \<a>\<r>\<r>\<a>\<y>[len] TY\<close>]
+                           distrib_right ucast_of_nat_small)
 \<medium_right_bracket> .
 
 
